Re-order prog_spec for better indentation

Shallow/ProgLang/Hoare.v
@@ -20,8 +20,8 @@ conditions and crash invariant specialized to a particular initial state. (This
 is why [pre] above is just a [Prop].) *)
 Definition Specification A T State := A -> State -> Quadruple T State.
 
-Definition prog_spec `(step: Semantics opT State)
-           A `(spec: Specification A T State) (p: prog opT T) :=
+Definition prog_spec A `(spec: Specification A T State) `(p: prog opT T)
+           `(step: Semantics opT State) :=
   forall a state,
     pre (spec a state) ->
     forall r, exec step p state r ->
@@ -50,8 +50,8 @@ Definition prog_double `(pre: DoublePre T State) `(p: prog opT T)
          | Crashed state' => crashinv state'
          end.
 
-Definition prog_ok `(step: Semantics opT State)
-           A `(spec: Specification A T State) (p: prog opT T) :=
+Definition prog_ok A `(spec: Specification A T State) `(p: prog opT T)
+           `(step: Semantics opT State) :=
   forall T' (rx: T -> prog opT T'),
     prog_double
       (fun state postcond crashinv =>
@@ -70,7 +70,7 @@ Theorem prog_ok_to_spec : forall `(step: Semantics opT State)
     (forall a state r state', pre (spec a state) ->
                  post (spec a state) r state' ->
                  crash (spec a state) state') ->
-    prog_ok step spec p -> prog_spec step spec p.
+    prog_ok spec p step -> prog_spec spec p step.
 Proof.
   unfold prog_ok, prog_double, prog_spec; intros.
   specialize (H0 _ Ret).
@@ -87,7 +87,7 @@ Qed.
 
 Theorem prog_spec_to_ok : forall `(step: Semantics opT State)
                             A `(spec: Specification A T State) (p: prog opT T),
-    prog_spec step spec p -> prog_ok step spec p.
+    prog_spec spec p step -> prog_ok spec p step.
 Proof.
   unfold prog_ok, prog_double, prog_spec; intros.
   deex.
@@ -104,7 +104,7 @@ Qed.
 Remark crash_invariants_must_handle_pre :
   forall `(step: Semantics opT State)
     A `(spec: Specification A T State) (p: prog opT T),
-    prog_spec step spec p ->
+    prog_spec spec p step ->
     forall a state, pre (spec a state) ->
            crash (spec a state) state.
 Proof.
